wip

isabelle/Distinct_Elems_While.thy
@@ -1,7 +1,6 @@
 theory Distinct_Elems_While
 
 imports
-  Probabilistic_While.While_SPMF
   CVM.Distinct_Elems_Algo
   CVM.Algo_Transforms_No_Fail
 
@@ -9,6 +8,19 @@ begin
 
 context with_threshold
 begin
+
+definition fix_state_while :: \<open>'a state \<Rightarrow> 'a state spmf\<close> where
+  \<open>fix_state_while \<equiv> loop_spmf.while (\<lambda> state.
+    card (state_chi state) = threshold) (\<lambda> state. do {
+      let chi = state_chi state;
+
+      keep_in_chi :: 'a \<Rightarrow> bool \<leftarrow>
+        prod_pmf chi \<lblot>bernoulli_pmf <| 1 / 2\<rblot>;
+
+      let chi = Set.filter keep_in_chi chi;
+      let k = state_k state + 1;
+
+      return_spmf \<lparr>state_k = k, state_chi = chi\<rparr>})\<close>
 
 definition step_while :: \<open>'a \<Rightarrow> 'a state \<Rightarrow> 'a state spmf\<close> where
   \<open>step_while x state \<equiv> do {
@@ -20,47 +32,62 @@ definition step_while :: \<open>'a \<Rightarrow> 'a state \<Rightarrow> 'a state
         then insert x
         else Set.remove x);
 
-    state\<lparr>state_chi := chi\<rparr>
-      |> loop_spmf.while (\<lambda> state.
-        card (state_chi state) \<ge> threshold) (\<lambda> state. do {
-          keep_in_chi :: 'a \<Rightarrow> bool \<leftarrow>
-            prod_pmf chi \<lblot>bernoulli_pmf <| 1 / 2\<rblot>;
-
-          let chi = Set.filter keep_in_chi (state_chi state);
-          let k = state_k state + 1;
-
-          return_spmf \<lparr>state_k = k, state_chi = chi\<rparr>}) }\<close>
+    fix_state_while (state\<lparr>state_chi := chi\<rparr>) }\<close>
 
 definition estimate_distinct_while :: \<open>'a list \<Rightarrow> nat spmf\<close> where
   \<open>estimate_distinct_while \<equiv> run_steps_then_estimate_spmf step_while\<close>
 
+end
+
+context with_threshold_pos
+begin
+
+lemma aux :
+  fixes state
+  defines \<open>chi \<equiv> state_chi state\<close>
+  assumes \<open>finite chi\<close> \<open>card chi \<le> threshold\<close>
+  shows
+    \<open>fix_state_while state = (
+      if card (state_chi state) < threshold
+      then return_spmf state
+      else do {
+        keep_in_chi :: 'a \<Rightarrow> bool \<leftarrow>
+          prod_pmf chi \<lblot>bernoulli_pmf <| 1 / 2\<rblot>;
+
+        let chi = Set.filter keep_in_chi chi;
+        let k = state_k state + 1;
+
+        fix_state_while \<lparr>state_k = k, state_chi = chi\<rparr> } )\<close>
+  unfolding fix_state_while_def Let_def
+  apply (subst bind_spmf_of_pmf[symmetric])+
+  apply (subst loop_spmf.while.simps)
+  apply (subst bind_spmf_assoc)
+  using assms by simp
+
 lemma
-  \<open>do {
-    state
-      |> loop_spmf.while (\<lambda> state.
-        card (state_chi state) \<ge> threshold) (\<lambda> state. do {
-          keep_in_chi :: 'a \<Rightarrow> bool \<leftarrow>
-            prod_pmf chi \<lblot>bernoulli_pmf <| 1 / 2\<rblot>;
+  assumes \<open>state ok\<close>
+  shows \<open>prob_fail (step_while x state) \<le> prob_fail (step x state)\<close>
+proof -
+  have \<open>\<turnstile>pmf
+    \<lbrakk>(\<lambda> state state'. state = state' \<and> (state ok))\<rbrakk>
+    \<langle>step x | step_while x\<rangle>
+    \<lbrakk>ord_option (=)\<rbrakk>\<close>
+    (is \<open>\<turnstile>pmf \<lbrakk>?R\<rbrakk> \<langle>_ | _ \<rangle> \<lbrakk>_\<rbrakk>\<close>)
+    unfolding step_def step_while_def Let_def Set.filter_def Set.remove_def 
+    apply (rule Utils_PMF_Relational.seq'[where S = \<open>(=)\<close>])
+    apply (simp add: Utils_PMF_Relational.relational_hoare_triple_def pmf.rel_refl)
+    apply (subst aux)
+    using assms
+    apply (auto simp add: well_formed_state_def Let_def card_insert_if)
+    apply (rule Utils_PMF_Relational.if_then_else)
+    apply simp_all
+    apply (rule Utils_PMF_Relational.seq'[where S = \<open>(=)\<close>])
+    by (auto
+      simp add: aux Set.filter_def fail_spmf_def Utils_PMF_Relational.relational_hoare_triple_def pmf.rel_refl)
 
-          let chi = Set.filter keep_in_chi (state_chi state);
-          let k = state_k state + 1;
-
-          return_spmf \<lparr>state_k = k, state_chi = chi\<rparr>}) }
-  = (
-    if card (state_chi state) < threshold
-    then return_spmf state
-    else do {
-      keep_in_chi :: 'a \<Rightarrow> bool \<leftarrow>
-        prod_pmf chi \<lblot>bernoulli_pmf <| 1 / 2\<rblot>;
-
-      let k = state_k state;
-      let chi = Set.filter keep_in_chi chi;
-
-      if card chi < threshold
-      then return_spmf \<lparr>state_k = k + 1, state_chi = chi\<rparr>
-      else fail_spmf
-    } )\<close>
-  sorry
+  then show ?thesis
+    using assms by (blast intro: prob_fail_le_of_relational_hoare_triple)
+qed
 
 end
 
